proof/array.v
@@ -11,14 +11,11 @@ Context (count: Int).
 
 Notation t := (TArray elem_ty count).
 
-
-Lemma valid_array {vs} (H: is_valid_for t (VTuple vs)) : Forall (fun v => is_valid_for elem_ty v) vs.
+Lemma array_dec {l v} (Hdec: decode t l = Some v) :
+exists vs, v = VTuple vs /\ Z.of_nat (length vs) = count.
 Proof.
-Admitted.
-
-
-Lemma array_encode_none {v} (H: encode t v = None) : ~is_valid_for t v.
-Proof.
+unfold decode in Hdec. fold decode in Hdec.
+unfold decode_array in Hdec.
 Admitted.
 
 Lemma encode_len {v ty l} (H: encode t v = Some l) : length l = ty_size ty.
@@ -33,94 +30,8 @@ Admitted.
 Lemma array_rt1 : rt1 t.
 Proof.
 intros Hwf v Hval.
-destruct (encode t v) as [l|] eqn:Henc; cycle 1. {
-  exfalso.
-  apply (array_encode_none Henc).
-  assumption.
-}
-
-exists l.
-split. { auto. }
-
-assert (exists vs, v = VTuple vs). {
-  unfold encode,encode_array in Henc.
-  destruct v; try (simpl in Henc; discriminate Henc).
-  eexists _. auto.
-}
-inversion H as [vs ->]. clear H.
-unfold decode. fold decode.
-unfold decode_array.
-simpl in Henc.
-unfold encode_array in Henc.
-simpl in Henc.
-unfold utils.assuming in Henc.
-
-destruct (BinInt.Z.eqb (BinInt.Z.of_nat (length vs)) count); cycle 1.
-{ simpl in Henc. discriminate Henc. }
-
-simpl in Henc.
-unfold utils.opt_bind in Henc.
-
-match goal with
-| _ : (utils.opt_map _ ?transp = Some _) |- _ => destruct transp eqn:Htransp
-end; cycle 1.
-{ simpl in Henc. discriminate Henc. }
- 
-simpl in Henc. inversion Henc. clear Henc H0 l.
-
-rewrite chunks_concat; cycle 1. { admit. }
-rewrite (transpose_map Htransp).
-
-assert (forall x l, encode elem_ty x = Some l -> (length l =? ty_size elem_ty) = true). { admit. }
-
-match goal with
-| |- (transpose (map ?f _) o-> _) = _ => replace f with (fun x => encode elem_ty x >>= decode elem_ty)
-end; cycle 1. {
-  apply functional_extensionality_dep.
-  intros v.
-  destruct (encode elem_ty v) eqn:E.
-  - rewrite (H v). auto. assumption.
-  - auto.
-}
-
-assert (transpose (map
- (fun x : Value => encode elem_ty x >>= decode elem_ty) vs) = Some vs); cycle 1.
-{ rewrite H0. simpl. auto. }
-
-have Hval' (valid_array Hval). clear Hval.
-
-generalize dependent l0.
-induction vs as [|v vs' IH].
-{ admit. }
-
-intros l0 Htransp.
-rewrite map_cons.
-
-assert (is_valid_for elem_ty v). { inversion Hval'. assumption. }
-assert (Hwf': wf elem_ty). { admit. }
-
-destruct (encode elem_ty v) eqn:E; cycle 1. {
-  simpl in Htransp.
-  rewrite E in Htransp.
-  discriminate Htransp.
-}
-
-assert (Hrt1 : rt1 elem_ty). { admit. }
-destruct (Hrt1 Hwf' v H0) as [ll [Henc Hdec]].
-assert (Hrew: ll = l). { rewrite Henc in E. inversion E. auto. }
-rewrite Hrew in Hdec,Henc. clear Hrew ll.
-rewrite bind_some.
-rewrite Hdec.
-rewrite transpose_some.
-
-destruct l0.
-{ (* discriminate within Htransp, left-side has length > 0, while right-side is []. *) admit. }
-
-assert (Forall (fun v : Value => is_valid_for elem_ty v) vs'). { inversion Hval'. assumption. }
-
-rewrite (IH H1 l1).
-- simpl. auto.
-- (* consequence of Htransp *) admit.
+destruct Hval as [l Hdec].
+destruct (array_dec Hdec) as [vs [-> Hcnt]].
 Admitted.
 
 Lemma array_rt2 : rt2 t.
